theories/Prelude/X.v
@@ -74,7 +74,7 @@ Qed.
 
 #[projections(primitive)]
 Class isFinite@{u} (A : Type@{u}) : Type@{u} :=
-  { finite_hasEqDec : hasEqDec@{u} A
+  { finite_hasEqDec : hasEqDec A
   ; finite_enumeration : list A
   ; finite_enumeration_complete
     : forall x : A, L.In x finite_enumeration
